Port Steel.Reference library to SteelSel

ulib/experimental/Steel.SelEffect.Atomic.fst
@@ -525,6 +525,14 @@ let intro_exists_erased #a #opened x p =
   rewrite_slprop (p x) (h_exists p)
     (fun m -> Steel.Memory.intro_h_exists (Ghost.reveal x) (fun x -> hp_of (p x)) m)
 
+let lift_exists #a #u p =
+  as_atomic_action_ghost (Steel.Memory.lift_h_exists #u (fun x -> hp_of (p x)))
+
+let exists_cong p q =
+  rewrite_slprop (h_exists p) (h_exists q)
+    (fun m -> Classical.forall_intro_2 reveal_equiv;
+            h_exists_cong (fun x -> hp_of (p x)) (fun x -> hp_of (q x)))
+
 let intro_vrefine v p =
   let m = get () in
   let x : Ghost.erased (t_of v) = gget v in
