ulib/experimental/Steel.SelReference.fst
@@ -17,10 +17,197 @@
 module Steel.SelReference
 
 open FStar.Ghost
+open Steel.Memory
 open Steel.SelEffect.Atomic
 open Steel.SelEffect
 module Mem = Steel.Memory
-module Eff = Steel.Effect
+module H = Steel.SelHigherReference
+module U = FStar.Universe
+
+#set-options "--ide_id_info_off"
+
+let ref a = H.ref (U.raise_t a)
+
+let null #a = H.null #(U.raise_t a)
+let is_null #a r = H.is_null #(U.raise_t a) r
+
+let pts_to_sl r p v = H.pts_to_sl r p (hide (U.raise_val (reveal v)))
+
+val raise_val_inj (#a:Type) (x y:a) : Lemma
+  (requires U.raise_val x == U.raise_val y)
+  (ensures x == y)
+
+let raise_val_inj x y =
+  U.downgrade_val_raise_val x;
+  U.downgrade_val_raise_val y
+
+
+let pts_to_ref_injective
+      (#a: Type u#0)
+      (r: ref a)
+      (p0 p1:perm)
+      (v0 v1: erased a)
+      (m:mem)
+    : Lemma
+      (requires
+        interp (pts_to_sl r p0 v0 `Mem.star` pts_to_sl r p1 v1) m)
+      (ensures v0 == v1)
+    = let v0' = hide (U.raise_val (reveal v0)) in
+      let v1' = hide (U.raise_val (reveal v1)) in
+      H.pts_to_ref_injective r p0 p1 v0' v1' m;
+      raise_val_inj (reveal v0) (reveal v1)
+
+let pts_to_not_null (#a:Type u#0)
+                    (x:ref a)
+                    (p:perm)
+                    (v: erased a)
+                    (m:mem)
+  : Lemma (requires interp (pts_to_sl x p v) m)
+          (ensures x =!= null)
+  = let v = hide (U.raise_val (reveal v)) in
+    H.pts_to_not_null #(U.raise_t a) x p v m
+
+// let pts_to_not_null' (#a:Type u#0)
+//                     (x:ref a)
+//                     (p:perm)
+//                     (v: erased a)
+//                     (m:mem)
+//                     (m1:mem{disjoint m m1})
+//   : Lemma (requires interp (pts_to_sl x p v) m)
+//           (ensures interp (pts_to_sl x p v) (Mem.join m m1))
+//   = ()
+
+
+let pts_to_witinv (#a:Type) (r:ref a) (p:perm) : Lemma (is_witness_invariant (pts_to_sl r p)) =
+  let aux (x y : erased a) (m:mem)
+    : Lemma (requires (interp (pts_to_sl r p x) m /\ interp (pts_to_sl r p y) m))
+            (ensures  (x == y))
+    = H.pts_to_witinv r p;
+      raise_val_inj (reveal x) (reveal y)
+  in
+  Classical.forall_intro_3 (fun x y -> Classical.move_requires (aux x y))
+
+let pts_to_injective_eq #a #opened #p0 #p1 #v0 #v1 r =
+  extract_info_raw (pts_to r p0 v0 `star` pts_to r p1 v1) (v0 == v1)
+    (fun m -> pts_to_ref_injective r p0 p1 v0 v1 m);
+  rewrite_slprop (pts_to r p1 v1) (pts_to r p1 v0) (fun _ -> ())
+
+let alloc_pt x =
+  let r = H.alloc (U.raise_val x) in
+  rewrite_slprop (H.pts_to r full_perm (U.raise_val x)) (pts_to r full_perm x) (fun _ -> ());
+  return r
+
+let read_pt #a #p #v r =
+  let v' = Ghost.hide (U.raise_val (Ghost.reveal v)) in
+  rewrite_slprop (pts_to r p v) (H.pts_to r p v') (fun _ -> ());
+  let x = H.read r in
+  let v':a = U.downgrade_val x in
+  rewrite_slprop (H.pts_to r p (hide x)) (pts_to r p v') (fun _ -> ());
+  return v'
+
+let read_refine_pt #a #p q r =
+  Classical.forall_intro_2 reveal_equiv;
+  lift_exists (fun (v:a) -> pts_to r p v `star` q v);
+  exists_cong (fun (v:U.raise_t a) -> pts_to r p (U.downgrade_val v) `star` q (U.downgrade_val v))
+                (fun (v:U.raise_t a) -> H.pts_to r p v `star` U.lift_dom q v);
+  let x = H.read_refine (U.lift_dom q) r in
+  rewrite_slprop
+    (H.pts_to r p (hide x) `star` U.lift_dom q x)
+    (pts_to r p (U.downgrade_val x) `star` q (U.downgrade_val x)) (fun _ -> ());
+
+  return (U.downgrade_val x)
+
+let write_pt #a #v r x =
+  let v' = Ghost.hide (U.raise_val (Ghost.reveal v)) in
+  rewrite_slprop (pts_to r full_perm v) (H.pts_to r full_perm v') (fun _ -> ());
+  let x' = U.raise_val x in
+  H.write r x';
+  rewrite_slprop (H.pts_to r full_perm (hide x')) (pts_to r full_perm x) (fun _ -> ())
+
+let free_pt #a #v r =
+  let v' = Ghost.hide (U.raise_val (Ghost.reveal v)) in
+  rewrite_slprop (pts_to r full_perm v) (H.pts_to r full_perm v') (fun _ -> ());
+  H.free r
+
+let share_pt #a #uses #p #v r =
+  let v' = Ghost.hide (U.raise_val (Ghost.reveal v)) in
+  rewrite_slprop (pts_to r p v) (H.pts_to r p v') (fun _ -> ());
+  H.share r;
+  rewrite_slprop (H.pts_to r (half_perm p) v') (pts_to r (half_perm p) v) (fun _ -> ());
+  rewrite_slprop (H.pts_to r (half_perm p) v') (pts_to r (half_perm p) v) (fun _ -> ())
+
+let hide_raise_reveal (#a:Type) (v0:erased a) (v1:erased a)
+  : Lemma (hide (U.raise_val (reveal v0)) == hide (U.raise_val (reveal v1)) <==>
+           v0 == v1)
+           [SMTPat (hide (U.raise_val (reveal v0)));
+            SMTPat (hide (U.raise_val (reveal v1)))]
+  = let u0 = hide (U.raise_val (reveal v0)) in
+    let u1 = hide (U.raise_val (reveal v1)) in
+    assert (U.downgrade_val (U.raise_val (reveal v0)) == U.downgrade_val (U.raise_val (reveal v1)) <==>
+            v0 == v1)
+
+let gather_pt #a #uses #p0 #p1 #v0 #v1 r =
+  let v0' = Ghost.hide (U.raise_val (Ghost.reveal v0)) in
+  let v1' = Ghost.hide (U.raise_val (Ghost.reveal v1)) in
+  rewrite_slprop (pts_to r p0 v0) (H.pts_to r p0 v0') (fun _ -> ());
+  rewrite_slprop (pts_to r p1 v1) (H.pts_to r p1 v1') (fun _ -> ());
+  let (u:unit{v0' == v1'}) = H.gather #_ #_ #p0 #p1 #v0' #v1' r in
+  rewrite_slprop (H.pts_to r (sum_perm p0 p1) v0') (pts_to r (sum_perm p0 p1) v0) (fun _ -> ());
+  u
+
+let raise_equiv (#t:Type) (x y:t)
+  : Lemma (U.raise_val x == U.raise_val y <==>
+           x == y)
+  = assert (U.downgrade_val (U.raise_val x) == x);
+    assert (U.downgrade_val (U.raise_val y) == y)
+
+
+let downgrade_equiv (#t:Type) (x y:U.raise_t t)
+  : Lemma (U.downgrade_val x == U.downgrade_val y <==>
+           x == y)
+  = assert (U.raise_val (U.downgrade_val x) == x);
+    assert (U.raise_val (U.downgrade_val y) == y)
+
+let lift_eq (#t:eqtype) (x y:U.raise_t t)
+  : b:bool{b <==> x==y}
+  = downgrade_equiv x y; U.downgrade_val x = U.downgrade_val y
+
+
+let cas_action (#t:eqtype)
+               (#uses:inames)
+               (r:ref t)
+               (v:Ghost.erased t)
+               (v_old:t)
+               (v_new:t)
+               (frame:slprop)
+   : MstTot (b:bool{b <==> (Ghost.reveal v == v_old)})
+             uses
+            (pts_to_sl r full_perm v)
+            (fun b -> if b then pts_to_sl r full_perm v_new else pts_to_sl r full_perm v)
+            frame
+            (fun _ -> True)
+            (fun _ _ _ -> True)
+   = let hv =     (Ghost.hide (U.raise_val (Ghost.reveal v))) in
+     let b = H.cas_action #(U.raise_t t)
+                  (lift_eq #t)
+                  #uses
+                  r
+                  hv
+                  (U.raise_val v_old)
+                  (U.raise_val v_new)
+                  frame
+     in
+     assert (b <==> (Ghost.reveal hv == U.raise_val v_old));
+     assert (b <==> U.raise_val (Ghost.reveal v) == U.raise_val v_old);
+     raise_equiv (Ghost.reveal v) v_old;
+     b
+
+let cas_pt #t #uses r v v_old v_new =
+  let b = as_atomic_action (cas_action #t #uses r v v_old v_new) in
+  rewrite_slprop (to_vprop (if b then pts_to_sl r full_perm v_new else pts_to_sl r full_perm v))
+                 (if b then pts_to r full_perm v_new else pts_to r full_perm v)
+                 (fun _ -> ());
+  return b
 
 (* Simple Reference library, only full permissions.
    AF: Permissions would likely need to be an index of the vprop ptr.
@@ -30,131 +217,90 @@ module Eff = Steel.Effect
    Refs on PCM are more complicated, and likely not usable with selectors
 *)
 
+let ptr r = Mem.h_exists (pts_to_sl r full_perm)
+
 val ptr_sel' (#a:Type0) (r: ref a) : selector' a (ptr r)
 let ptr_sel' #a r = fun h ->
-  let x = id_elim_exists #(erased a) (R.pts_to r full_perm) h in
+  let x = id_elim_exists #(erased a) (pts_to_sl r full_perm) h in
   reveal (reveal x)
+
+let join_preserves_interp (hp:slprop) (m0:hmem hp) (m1:mem{disjoint m0 m1})
+: Lemma
+  (interp hp (join m0 m1))
+  [SMTPat (interp hp (join m0 m1))]
+= let open Steel.Memory in
+  intro_emp m1;
+  intro_star hp emp m0 m1;
+  affine_star hp emp (join m0 m1)
 
 let ptr_sel_depends_only_on (#a:Type0) (r:ref a)
   (m0:Mem.hmem (ptr r)) (m1:mem{disjoint m0 m1})
   : Lemma (ptr_sel' r m0 == ptr_sel' r (Mem.join m0 m1))
-  = let x = reveal (id_elim_exists #(erased a) (R.pts_to r full_perm) m0) in
-    let y = reveal (id_elim_exists #(erased a) (R.pts_to r full_perm) (Mem.join m0 m1)) in
-    R.pts_to_witinv r full_perm;
-    elim_wi (R.pts_to r full_perm) x y (Mem.join m0 m1)
+  = let x = reveal (id_elim_exists #(erased a) (pts_to_sl r full_perm) m0) in
+    let y = reveal (id_elim_exists #(erased a) (pts_to_sl r full_perm) (Mem.join m0 m1)) in
+    pts_to_witinv r full_perm;
+    elim_wi (pts_to_sl r full_perm) x y (Mem.join m0 m1)
 
 let ptr_sel_depends_only_on_core (#a:Type0) (r:ref a)
   (m0:Mem.hmem (ptr r))
   : Lemma (ptr_sel' r m0 == ptr_sel' r (core_mem m0))
-  = let x = reveal (id_elim_exists #(erased a) (R.pts_to r full_perm) m0) in
-    let y = reveal (id_elim_exists #(erased a) (R.pts_to r full_perm) (core_mem m0)) in
-    R.pts_to_witinv r full_perm;
-    elim_wi (R.pts_to r full_perm) x y (core_mem m0)
+  = let x = reveal (id_elim_exists #(erased a) (pts_to_sl r full_perm) m0) in
+    let y = reveal (id_elim_exists #(erased a) (pts_to_sl r full_perm) (core_mem m0)) in
+    pts_to_witinv r full_perm;
+    elim_wi (pts_to_sl r full_perm) x y (core_mem m0)
 
 let ptr_sel r =
   Classical.forall_intro_2 (ptr_sel_depends_only_on r);
   Classical.forall_intro (ptr_sel_depends_only_on_core r);
   ptr_sel' r
 
-let ptr_sel_interp #a r m = R.pts_to_witinv r full_perm
+let ptr_sel_interp #a r m = pts_to_witinv r full_perm
 
-friend Steel.Effect
-friend Steel.SelEffect
+let intro_vptr_lemma (#a:Type) (r:ref a) (v:erased a) (m:mem) : Lemma
+  (requires interp (pts_to_sl r full_perm v) m)
+  (ensures interp (ptr r) m /\ ptr_sel r m == reveal v)
+  = Mem.intro_h_exists v (pts_to_sl r full_perm) m;
+    pts_to_witinv r full_perm
 
-let as_steelsel0 (#a:Type)
-  (#pre:pre_t) (#post:post_t a)
-  (#req:prop) (#ens:a -> prop)
-  ($f:Eff.repr a false (hp_of pre) (fun x -> hp_of (post x)) (fun h -> req) (fun _ x _ -> ens x))
-: repr a false pre post (fun _ -> req) (fun _ x _ -> ens x)
-  = fun frame -> f frame
+let elim_vptr_lemma (#a:Type) (r:ref a) (v:erased a) (m:mem) : Lemma
+  (requires interp (ptr r) m /\ ptr_sel r m == reveal v)
+  (ensures interp (pts_to_sl r full_perm v) m)
+  = Mem.elim_h_exists (pts_to_sl r full_perm) m;
+    pts_to_witinv r full_perm
 
-let as_steelsel1 (#a:Type)
-  (#pre:vprop) (#post:a -> vprop)
-  (#req:prop) (#ens:a -> prop)
-  ($f:Eff.repr a false (hp_of pre) (fun x -> hp_of (post x)) (fun h -> req) (fun _ x _ -> ens x))
-: SteelSel a pre post (fun _ -> req) (fun _ x _ -> ens x)
-  = SteelSel?.reflect (as_steelsel0 f)
+let intro_vptr (#a:Type) (#opened:inames) (r:ref a) (v:erased a)
+  : SteelSelGhost unit opened (pts_to r full_perm v) (fun _ -> vptr r)
+                       (requires fun _ -> True)
+                       (ensures fun _ _ h1 -> sel r h1 == reveal v)
+  = change_slprop_2 (pts_to r full_perm v) (vptr r) v (intro_vptr_lemma r v)
 
-let as_steelsel (#a:Type)
-  (#pre:pre_t) (#post:post_t a)
-  (#req:prop) (#ens:a -> prop)
-  ($f:unit -> Eff.Steel a (hp_of pre) (fun x -> hp_of (post x)) (fun h -> req) (fun _ x _ -> ens x))
-: SteelSel a pre post (fun _ -> req) (fun _ x _ -> ens x)
-  = as_steelsel1 (Steel.Effect.reify_steel_comp f)
-
-let _:squash (hp_of emp == Mem.emp /\ t_of emp == unit) = reveal_emp ()
-
-unfold
-let vptr_tmp' (#a:Type) (r:ref a) (p:perm) (v:erased a) : vprop' =
-  { hp = R.pts_to r p v;
-    t = unit;
-    sel = fun _ -> ()}
-unfold
-let vptr_tmp r p v : vprop = VUnit (vptr_tmp' r p v)
-
-val alloc0 (#a:Type0) (x:a) : SteelSel (ref a)
-  emp (fun r -> vptr_tmp r full_perm x)
-  (requires fun _ -> True)
-  (ensures fun _ r h1 -> True)
-
-let alloc0 #a x = as_steelsel (fun _ -> R.alloc x)
-
-let intro_vptr (#a:Type) (r:ref a) (v:erased a) (m:mem) : Lemma
-  (requires interp (hp_of (vptr_tmp r full_perm v)) m)
-  (ensures interp (hp_of (vptr r)) m /\ sel_of (vptr r) m == reveal v)
-  = Mem.intro_h_exists v (R.pts_to r full_perm) m;
-    R.pts_to_witinv r full_perm
-
-let elim_vptr (#a:Type) (r:ref a) (v:erased a) (m:mem) : Lemma
-  (requires interp (hp_of (vptr r)) m /\ sel_of (vptr r) m == reveal v)
-  (ensures interp (hp_of (vptr_tmp r full_perm v)) m)
-  = Mem.elim_h_exists (R.pts_to r full_perm) m;
-    R.pts_to_witinv r full_perm
+let elim_vptr (#a:Type) (#opened:inames) (r:ref a)
+  : SteelSelGhost (erased a) opened (vptr r) (fun v -> pts_to r full_perm v)
+                       (requires fun _ -> True)
+                       (ensures fun h0 v _ -> reveal v == sel r h0)
+  = let v = gget (vptr r) in
+    change_slprop (vptr r) (pts_to r full_perm v) v () (elim_vptr_lemma r v);
+    v
 
 let alloc x =
-  let r = alloc0 x in
-  extract_info (vptr_tmp r full_perm x) () (~ (R.is_null r))
-    (fun m -> R.pts_to_not_null r full_perm x m);
-  change_slprop (vptr_tmp r full_perm x) (vptr r) () x (intro_vptr r x);
+  let r = alloc_pt x in
+  intro_vptr r (hide x);
   return r
 
-let free r = change_slprop_2 (vptr r) emp () intro_emp
+let free r =
+  let _ = elim_vptr r in
+  free_pt r
 
-val read0 (#a:Type0) (r:ref a) (v:erased a) : SteelSel a
-  (vptr_tmp r full_perm v) (fun x -> vptr_tmp r full_perm x)
-  (requires fun _ -> True)
-  (ensures fun h0 x h1 -> x == reveal v)
+let read r =
+  let _ = elim_vptr r in
+  let x = read_pt r in
+  intro_vptr r x;
+  return x
 
-let read0 #a r v = as_steelsel (fun _ -> R.read #a #full_perm #v r)
-
-let read (#a:Type0) (r:ref a) : SteelSel a
-  (vptr r) (fun _ -> vptr r)
-  (requires fun _ -> True)
-  (ensures fun h0 x h1 -> h0 (vptr r) == h1 (vptr r) /\ x == h1 (vptr r))
-  = let h0 = get() in
-    let v = hide ((reveal h0) (vptr r)) in
-    change_slprop (vptr r) (vptr_tmp r full_perm v) v () (elim_vptr r v);
-    let x = read0 r v in
-    change_slprop (vptr_tmp r full_perm x) (vptr r) () x (intro_vptr r x);
-    return x
-
-val write0 (#a:Type0) (v:erased a) (r:ref a) (x:a)
-  : SteelSel unit
-    (vptr_tmp r full_perm v) (fun _ -> vptr_tmp r full_perm x)
-    (fun _ -> True) (fun _ _ _ -> True)
-
-let write0 #a v r x = as_steelsel (fun _ -> R.write #a #v r x)
-
-let write (#a:Type0) (r:ref a) (x:a) : SteelSel unit
-  (vptr r) (fun _ -> vptr r)
-  (requires fun _ -> True)
-  (ensures fun _ _ h1 -> x == h1 (vptr r))
-  = let h0 = get() in
-    let v = hide ((reveal h0) (vptr r)) in
-    change_slprop (vptr r) (vptr_tmp r full_perm v) v () (elim_vptr r v);
-    write0 v r x;
-    change_slprop (vptr_tmp r full_perm x) (vptr r) () x (intro_vptr r x)
-
+let write r x =
+  let _ = elim_vptr r in
+  write_pt r x;
+  intro_vptr r x
 
 (*** Lemmas on references *)
 
@@ -163,107 +309,151 @@ let vptr_not_null
 = change_slprop_rel
     (vptr r)
     (vptr r)
-    (fun x y -> x == y /\ R.is_null r == false)
-    (fun m -> R.pts_to_not_null r full_perm (ptr_sel r m) m)
+    (fun x y -> x == y /\ is_null r == false)
+    (fun m -> pts_to_not_null r full_perm (ptr_sel r m) m)
 
 (*** Ghost pointers *)
 
+(*** GHOST REFERENCES ***)
+let ghost_ref a = H.ghost_ref (U.raise_t a)
+
+let raise_erased (#a:Type0) (x:erased a)
+  : erased (U.raise_t u#0 u#1 a)
+  = Ghost.hide (U.raise_val (Ghost.reveal x))
+
+[@__reduce__]
+let ghost_pts_to_sl #a r p x = H.ghost_pts_to_sl #(U.raise_t a) r p (raise_erased x)
+
+let ghost_pts_to_witinv (#a:Type) (r:ghost_ref a) (p:perm) : Lemma (is_witness_invariant (ghost_pts_to_sl r p)) =
+  let aux (x y : erased a) (m:mem)
+    : Lemma (requires (interp (ghost_pts_to_sl r p x) m /\ interp (ghost_pts_to_sl r p y) m))
+            (ensures  (x == y))
+    = H.ghost_pts_to_witinv r p;
+      raise_val_inj (reveal x) (reveal y)
+  in
+  Classical.forall_intro_3 (fun x y -> Classical.move_requires (aux x y))
+
+let ghost_alloc_pt (#a:Type) (#u:_) (x:erased a)
+  : SteelSelGhostT (ghost_ref a) u
+    emp
+    (fun r -> ghost_pts_to r full_perm x)
+  = H.ghost_alloc (raise_erased x)
+
+let ghost_free_pt r = H.ghost_free r
+
+let ghost_share_pt (#a:Type) (#u:_)
+                (#p:perm)
+                (#x:erased a)
+                (r:ghost_ref a)
+   = H.ghost_share r
+
+let ghost_gather_pt (#a:Type) (#u:_)
+                 (#p0 #p1:perm)
+                 (#x0 #x1:erased a)
+                 (r:ghost_ref a)
+  : SteelSelGhost unit u
+    (ghost_pts_to r p0 x0 `star`
+     ghost_pts_to r p1 x1)
+    (fun _ -> ghost_pts_to r (sum_perm p0 p1) x0)
+    (requires fun _ -> true)
+    (ensures fun _ _ _ -> x0 == x1)
+  = H.ghost_gather r
+
+let ghost_pts_to_injective_eq (#a:_) (#u:_) (#p #q:_) (r:ghost_ref a) (v0 v1:Ghost.erased a)
+  : SteelSelGhost unit u
+    (ghost_pts_to r p v0 `star` ghost_pts_to r q v1)
+    (fun _ -> ghost_pts_to r p v0 `star` ghost_pts_to r q v0)
+    (requires fun _ -> True)
+    (ensures fun _ _ _ -> v0 == v1)
+  = H.ghost_pts_to_injective_eq r (raise_erased v0) (raise_erased v1)
+
+let ghost_read_pt #a #u #p #v r =
+  let x = H.ghost_read r in
+  let x' = hide (U.downgrade_val (reveal x)) in
+  rewrite_slprop (H.ghost_pts_to r p x) (ghost_pts_to r p x') (fun _ -> ());
+  x'
+
+let ghost_write_pt (#a:Type) (#u:_) (#v:erased a) (r:ghost_ref a) (x:erased a)
+  : SteelSelGhostT unit u
+    (ghost_pts_to r full_perm v)
+    (fun _ -> ghost_pts_to r full_perm x)
+  = H.ghost_write r (raise_erased x)
+
+(* Selector version of ghost pointers *)
+
+let ghost_ptr r = Mem.h_exists (ghost_pts_to_sl r full_perm)
+
 val ghost_ptr_sel' (#a:Type0) (r: ghost_ref a) : selector' a (ghost_ptr r)
 let ghost_ptr_sel' #a r = fun h ->
-  let x = id_elim_exists #(erased a) (R.ghost_pts_to r full_perm) h in
+  let x = id_elim_exists #(erased a) (ghost_pts_to_sl r full_perm) h in
   reveal (reveal x)
 
 let ghost_ptr_sel_depends_only_on (#a:Type0) (r:ghost_ref a)
   (m0:Mem.hmem (ghost_ptr r)) (m1:mem{disjoint m0 m1})
   : Lemma (ghost_ptr_sel' r m0 == ghost_ptr_sel' r (Mem.join m0 m1))
-  = let x = reveal (id_elim_exists #(erased a) (R.ghost_pts_to r full_perm) m0) in
-    let y = reveal (id_elim_exists #(erased a) (R.ghost_pts_to r full_perm) (Mem.join m0 m1)) in
-    R.ghost_pts_to_witinv r full_perm;
-    elim_wi (R.ghost_pts_to r full_perm) x y (Mem.join m0 m1)
+  = let x = reveal (id_elim_exists #(erased a) (ghost_pts_to_sl r full_perm) m0) in
+    let y = reveal (id_elim_exists #(erased a) (ghost_pts_to_sl r full_perm) (Mem.join m0 m1)) in
+    ghost_pts_to_witinv r full_perm;
+    elim_wi (ghost_pts_to_sl r full_perm) x y (Mem.join m0 m1)
 
 let ghost_ptr_sel_depends_only_on_core (#a:Type0) (r:ghost_ref a)
   (m0:Mem.hmem (ghost_ptr r))
   : Lemma (ghost_ptr_sel' r m0 == ghost_ptr_sel' r (core_mem m0))
-  = let x = reveal (id_elim_exists #(erased a) (R.ghost_pts_to r full_perm) m0) in
-    let y = reveal (id_elim_exists #(erased a) (R.ghost_pts_to r full_perm) (core_mem m0)) in
-    R.ghost_pts_to_witinv r full_perm;
-    elim_wi (R.ghost_pts_to r full_perm) x y (core_mem m0)
+  = let x = reveal (id_elim_exists #(erased a) (ghost_pts_to_sl r full_perm) m0) in
+    let y = reveal (id_elim_exists #(erased a) (ghost_pts_to_sl r full_perm) (core_mem m0)) in
+    ghost_pts_to_witinv r full_perm;
+    elim_wi (ghost_pts_to_sl r full_perm) x y (core_mem m0)
 
 let ghost_ptr_sel r =
   Classical.forall_intro_2 (ghost_ptr_sel_depends_only_on r);
   Classical.forall_intro (ghost_ptr_sel_depends_only_on_core r);
   ghost_ptr_sel' r
 
-let ghost_ptr_sel_interp #a r m = R.ghost_pts_to_witinv r full_perm
+let ghost_ptr_sel_interp #a r m = ghost_pts_to_witinv r full_perm
 
-friend Steel.Effect.Atomic
-friend Steel.SelEffect.Atomic
-module Eff = Steel.Effect.Atomic
 
-let as_steelselghost0 (#a:Type) (#opened: _)
-  (#pre:pre_t) (#post:post_t a)
-  (#req:prop) (#ens:a -> prop)
-  ($f:Eff.repr a false opened Eff.Unobservable (hp_of pre) (fun x -> hp_of (post x)) (fun h -> req) (fun _ x _ -> ens x))
-: Steel.SelEffect.Atomic.repr a false opened Unobservable pre post (fun _ -> req) (fun _ x _ -> ens x)
-  = fun frame -> f frame
+let intro_ghost_vptr_lemma (#a:Type) (r:ghost_ref a) (v:erased a) (m:mem) : Lemma
+  (requires interp (ghost_pts_to_sl r full_perm v) m)
+  (ensures interp (ghost_ptr r) m /\ ghost_ptr_sel r m == reveal v)
+  = Mem.intro_h_exists v (ghost_pts_to_sl r full_perm) m;
+    ghost_pts_to_witinv r full_perm
 
-let as_steelselghost1 (#a:Type) (#opened: _)
-  (#pre:vprop) (#post:a -> vprop)
-  (#req:prop) (#ens:a -> prop)
-  ($f:Eff.repr a false opened Eff.Unobservable (hp_of pre) (fun x -> hp_of (post x)) (fun h -> req) (fun _ x _ -> ens x))
-: SteelSelGhost a opened pre post (fun _ -> req) (fun _ x _ -> ens x)
-  = SteelSelGhost?.reflect (as_steelselghost0 f)
+let elim_ghost_vptr_lemma (#a:Type) (r:ghost_ref a) (v:erased a) (m:mem) : Lemma
+  (requires interp (ghost_ptr r) m /\ ghost_ptr_sel r m == reveal v)
+  (ensures interp (ghost_pts_to_sl r full_perm v) m)
+  = Mem.elim_h_exists (ghost_pts_to_sl r full_perm) m;
+    ghost_pts_to_witinv r full_perm
 
-let as_steelselghost (#a:Type) (#opened: _)
-  (#pre:pre_t) (#post:post_t a)
-  (#req:prop) (#ens:a -> prop)
-  ($f:unit -> Eff.SteelGhost a opened (hp_of pre) (fun x -> hp_of (post x)) (fun h -> req) (fun _ x _ -> ens x))
-: SteelSelGhost a opened pre post (fun _ -> req) (fun _ x _ -> ens x)
-  = as_steelselghost1 (Steel.Effect.Atomic.reify_steel_ghost_comp f)
+let intro_ghost_vptr (#a:Type) (#opened:inames) (r:ghost_ref a) (v:erased a)
+  : SteelSelGhost unit opened (ghost_pts_to r full_perm v) (fun _ -> ghost_vptr r)
+                       (requires fun _ -> True)
+                       (ensures fun _ _ h1 -> ghost_sel r h1 == reveal v)
+  = change_slprop_2 (ghost_pts_to r full_perm v) (ghost_vptr r) v (intro_ghost_vptr_lemma r v)
 
-unfold
-let ghost_vptr_tmp' (#a:Type) (r:ghost_ref a) (p:perm) (v:erased a) : vprop' =
-  { hp = R.ghost_pts_to r p v;
-    t = unit;
-    sel = fun _ -> ()}
-unfold
-let ghost_vptr_tmp r p v : vprop = VUnit (ghost_vptr_tmp' r p v)
-
-val ghost_alloc0 (#a:Type0) (#opened: _) (x:a) : SteelSelGhost (ghost_ref a) opened
-  emp (fun r -> ghost_vptr_tmp r full_perm x)
-  (requires fun _ -> True)
-  (ensures fun _ r h1 -> True)
-
-let ghost_alloc0 #a x = as_steelselghost (fun _ -> R.ghost_alloc x)
-
-let intro_ghost_vptr (#a:Type) (r:ghost_ref a) (v:erased a) (m:mem) : Lemma
-  (requires interp (hp_of (ghost_vptr_tmp r full_perm v)) m)
-  (ensures interp (hp_of (ghost_vptr r)) m /\ sel_of (ghost_vptr r) m == reveal v)
-  = Mem.intro_h_exists v (R.ghost_pts_to r full_perm) m;
-    R.ghost_pts_to_witinv r full_perm
-
-let elim_ghost_vptr (#a:Type) (r:ghost_ref a) (v:erased a) (m:mem) : Lemma
-  (requires interp (hp_of (ghost_vptr r)) m /\ sel_of (ghost_vptr r) m == reveal v)
-  (ensures interp (hp_of (ghost_vptr_tmp r full_perm v)) m)
-  = Mem.elim_h_exists (R.ghost_pts_to r full_perm) m;
-    R.ghost_pts_to_witinv r full_perm
+let elim_ghost_vptr (#a:Type) (#opened:inames) (r:ghost_ref a)
+  : SteelSelGhost (erased a) opened (ghost_vptr r) (fun v -> ghost_pts_to r full_perm v)
+                       (requires fun _ -> True)
+                       (ensures fun h0 v _ -> reveal v == ghost_sel r h0)
+  = let v = gget (ghost_vptr r) in
+    change_slprop (ghost_vptr r) (ghost_pts_to r full_perm v) v () (elim_ghost_vptr_lemma r v);
+    v
 
 let ghost_alloc x =
-  let r = ghost_alloc0 (Ghost.reveal x) in
-  change_slprop (ghost_vptr_tmp r full_perm (Ghost.reveal x)) (ghost_vptr r) () x (intro_ghost_vptr r x);
+  let r = ghost_alloc_pt x in
+  intro_ghost_vptr r x;
   r
 
-let ghost_free r = change_slprop_rel (ghost_vptr r) emp (fun _ _ -> True) intro_emp
+let ghost_free r =
+  let _ = elim_ghost_vptr r in
+  ghost_free_pt r
 
-val ghost_write0 (#a:Type0) (#opened: _) (v:erased a) (r:ghost_ref a) (x:a)
-  : SteelSelGhost unit opened
-    (ghost_vptr_tmp r full_perm v) (fun _ -> ghost_vptr_tmp r full_perm x)
-    (fun _ -> True) (fun _ _ _ -> True)
+let ghost_read r =
+  let _ = elim_ghost_vptr r in
+  let x = ghost_read_pt r in
+  intro_ghost_vptr r x;
+  x
 
-let ghost_write0 #a #opened v r x = as_steelselghost (fun _ -> R.ghost_write #a #opened #v r x)
-
-let ghost_write r x
-  = let v = gget (ghost_vptr r) in
-    change_slprop (ghost_vptr r) (ghost_vptr_tmp r full_perm v) v () (elim_ghost_vptr r v);
-    ghost_write0 v r (Ghost.reveal x);
-    change_slprop (ghost_vptr_tmp r full_perm (Ghost.reveal x)) (ghost_vptr r) () x (intro_ghost_vptr r x)
+let ghost_write r x =
+  let _ = elim_ghost_vptr r in
+  ghost_write_pt r x;
+  intro_ghost_vptr r x
