ulib/experimental/Steel.SelReference.fsti
@@ -16,22 +16,114 @@
 
 module Steel.SelReference
 
+open FStar.Ghost
+open Steel.FractionalPermission
+
 open Steel.Memory
 open Steel.SelEffect.Atomic
 open Steel.SelEffect
 
-module R = Steel.Reference
 module Mem = Steel.Memory
-open Steel.FractionalPermission
 
-let ref (a:Type0) : Type0 = R.ref a
-let ptr (#a:Type0) (r:ref a) : slprop u#1 = Mem.h_exists (R.pts_to r full_perm)
+val ref (a:Type0) : Type0
+
+val null (#a:Type0) : ref a
+val is_null (#a:Type0) (r:ref a) : (b:bool{b <==> r == null})
+
+(* Standard separation logic assertion *)
+
+val pts_to_sl (#a:Type0) (r:ref a) (p:perm) (v:erased a) : slprop u#1
+
+[@@ __steel_reduce__]
+unfold let pts_to (#a:Type0) (r:ref a) ([@@@smt_fallback] p:perm) ([@@@ smt_fallback] v:erased a)
+  = to_vprop (pts_to_sl r p v)
+
+val pts_to_ref_injective
+      (#a: Type u#0)
+      (r: ref a)
+      (p0 p1:perm)
+      (v0 v1: erased a)
+      (m:mem)
+    : Lemma
+      (requires
+        interp (pts_to_sl r p0 v0 `Mem.star` pts_to_sl r p1 v1) m)
+      (ensures v0 == v1)
+
+val pts_to_not_null (#a:Type u#0)
+                    (x:ref a)
+                    (p:perm)
+                    (v: erased a)
+                    (m:mem)
+  : Lemma (requires interp (pts_to_sl x p v) m)
+          (ensures x =!= null)
+
+val pts_to_witinv (#a:Type) (r:ref a) (p:perm) : Lemma (is_witness_invariant (pts_to_sl r p))
+
+val pts_to_injective_eq
+      (#a: Type)
+      (#opened:inames)
+      (#p0 #p1:perm)
+      (#v0 #v1: erased a)
+      (r: ref a)
+  : SteelSelGhost unit opened
+          (pts_to r p0 v0 `star` pts_to r p1 v1)
+          (fun _ -> pts_to r p0 v0 `star` pts_to r p1 v0)
+          (requires fun _ -> True)
+          (ensures fun _ _ _ -> v0 == v1)
+
+val alloc_pt (#a:Type) (x:a)
+  : SteelSel (ref a) emp (fun r -> pts_to r full_perm x)
+             (requires fun _ -> True)
+             (ensures fun _ r _ -> not (is_null r))
+
+val read_pt (#a:Type) (#p:perm) (#v:erased a) (r:ref a)
+  : SteelSel a (pts_to r p v) (fun x -> pts_to r p x)
+           (requires fun _ -> True)
+           (ensures fun _ x _ -> x == Ghost.reveal v)
+
+val read_refine_pt (#a:Type0) (#p:perm) (q:a -> vprop) (r:ref a)
+  : SteelSelT a (h_exists (fun (v:a) -> pts_to r p v `star` q v))
+             (fun v -> pts_to r p v `star` q v)
+
+val write_pt (#a:Type0) (#v:erased a) (r:ref a) (x:a)
+  : SteelSelT unit (pts_to r full_perm v) (fun _ -> pts_to r full_perm x)
+
+val free_pt (#a:Type0) (#v:erased a) (r:ref a)
+  : SteelSelT unit (pts_to r full_perm v) (fun _ -> emp)
+
+val share_pt (#a:Type0) (#uses:_) (#p:perm) (#v:erased a) (r:ref a)
+  : SteelSelGhostT unit uses
+    (pts_to r p v)
+    (fun _ -> pts_to r (half_perm p) v `star` pts_to r (half_perm p) v)
+
+val gather_pt (#a:Type0) (#uses:_) (#p0:perm) (#p1:perm) (#v0 #v1:erased a) (r:ref a)
+  : SteelSelGhostT (_:unit{v0 == v1}) uses
+    (pts_to r p0 v0 `star` pts_to r p1 v1)
+    (fun _ -> pts_to r (sum_perm p0 p1) v0)
+
+val cas_pt (#t:eqtype)
+        (#uses:inames)
+        (r:ref t)
+        (v:Ghost.erased t)
+        (v_old:t)
+        (v_new:t)
+  : SteelSelAtomicT
+        (b:bool{b <==> (Ghost.reveal v == v_old)})
+        uses
+        (pts_to r full_perm v)
+        (fun b -> if b then pts_to r full_perm v_new else pts_to r full_perm v)
+
+(* Ptr version with a selector *)
+
+(* AF: TODO: Should be indexed by a perm *)
+
+val ptr (#a:Type0) (r:ref a) : slprop u#1
 
 val ptr_sel (#a:Type0) (r:ref a) : selector a (ptr r)
 
 val ptr_sel_interp (#a:Type0) (r:ref a) (m:mem) : Lemma
   (requires interp (ptr r) m)
-  (ensures interp (R.pts_to r full_perm (ptr_sel r m)) m)
+  (ensures interp (pts_to_sl r full_perm (ptr_sel r m)) m)
 
 [@@ __steel_reduce__]
 let vptr' #a r : vprop' =
@@ -43,10 +135,15 @@ let vptr' #a r : vprop' =
 unfold
 let vptr r = VUnit (vptr' r)
 
+[@@ __steel_reduce__]
+let sel (#a:Type) (#p:vprop) (r:ref a)
+  (h:rmem p{FStar.Tactics.with_tactic selector_tactic (can_be_split p (vptr r) /\ True)})
+  = h (vptr r)
+
 val alloc (#a:Type0) (x:a) : SteelSel (ref a)
   emp (fun r -> vptr r)
   (requires fun _ -> True)
-  (ensures fun _ r h1 -> h1 (vptr r) == x /\ not (R.is_null r))
+  (ensures fun _ r h1 -> sel r h1 == x /\ not (is_null r))
 
 val free (#a:Type0) (r:ref a) : SteelSel unit
   (vptr r) (fun _ -> emp)
@@ -56,41 +153,99 @@ val free (#a:Type0) (r:ref a) : SteelSel unit
 val read (#a:Type0) (r:ref a) : SteelSel a
   (vptr r) (fun _ -> vptr r)
   (requires fun _ -> True)
-  (ensures fun h0 x h1 -> h0 (vptr r) == h1 (vptr r) /\ x == h1 (vptr r))
+  (ensures fun h0 x h1 -> sel r h0 == sel r h1 /\ x == sel r h1)
 
 val write (#a:Type0) (r:ref a) (x:a) : SteelSel unit
   (vptr r) (fun _ -> vptr r)
   (requires fun _ -> True)
-  (ensures fun _ _ h1 -> x == h1 (vptr r))
+  (ensures fun _ _ h1 -> x == sel r h1)
 
 val vptr_not_null (#opened: _)
   (#a: Type)
-  (r: R.ref a)
+  (r: ref a)
 : SteelSelGhost unit opened
     (vptr r)
     (fun _ -> vptr r)
     (fun _ -> True)
     (fun h0 _ h1 ->
-      h1 (vptr r) == h0 (vptr r) /\
-      R.is_null r == false
+      sel r h0 == sel r h1 /\
+      is_null r == false
     )
-
-[@@ __steel_reduce__]
-let sel (#a:Type) (#p:vprop) (r:ref a)
-  (h:rmem p{FStar.Tactics.with_tactic selector_tactic (can_be_split p (vptr r) /\ True)})
-  = h (vptr r)
 
 (*** Ghost references ***)
 
 [@@ erasable]
-let ghost_ref (a:Type u#0) : Type u#0 = R.ghost_ref a
-let ghost_ptr (#a: Type0) (r: ghost_ref a) : Tot (slprop u#1) = Mem.h_exists (R.ghost_pts_to r full_perm)
+val ghost_ref (a:Type u#0) : Type u#0
+
+(* Textbook separation logic version of ghost references *)
+
+val ghost_pts_to_sl (#a:_) (r:ghost_ref a) (p:perm) (v:erased a) : slprop u#1
+
+[@@ __steel_reduce__]
+unfold let ghost_pts_to (#a:Type0)
+  (r:ghost_ref a)
+  ([@@@smt_fallback] p:perm)
+  ([@@@ smt_fallback] v:erased a)
+  : vprop
+  = to_vprop (ghost_pts_to_sl r p v)
+
+val ghost_pts_to_witinv (#a:Type) (r:ghost_ref a) (p:perm)
+  : Lemma (is_witness_invariant (ghost_pts_to_sl r p))
+
+val ghost_alloc_pt (#a:Type) (#u:_) (x:erased a)
+  : SteelSelGhostT (ghost_ref a) u
+    emp
+    (fun r -> ghost_pts_to r full_perm x)
+
+val ghost_free_pt (#a:Type0) (#u:_) (#v:erased a) (r:ghost_ref a)
+  : SteelSelGhostT unit u (ghost_pts_to r full_perm v) (fun _ -> emp)
+
+val ghost_share_pt (#a:Type) (#u:_)
+                (#p:perm)
+                (#x:erased a)
+                (r:ghost_ref a)
+  : SteelSelGhostT unit u
+    (ghost_pts_to r p x)
+    (fun _ -> ghost_pts_to r (half_perm p) x `star`
+           ghost_pts_to r (half_perm p) x)
+
+val ghost_gather_pt (#a:Type) (#u:_)
+                 (#p0 #p1:perm)
+                 (#x0 #x1:erased a)
+                 (r:ghost_ref a)
+  : SteelSelGhost unit u
+    (ghost_pts_to r p0 x0 `star`
+     ghost_pts_to r p1 x1)
+    (fun _ -> ghost_pts_to r (sum_perm p0 p1) x0)
+    (requires fun _ -> true)
+    (ensures fun _ _ _ -> x0 == x1)
+
+val ghost_pts_to_injective_eq (#a:_) (#u:_) (#p #q:_) (r:ghost_ref a) (v0 v1:Ghost.erased a)
+  : SteelSelGhost unit u
+    (ghost_pts_to r p v0 `star` ghost_pts_to r q v1)
+    (fun _ -> ghost_pts_to r p v0 `star` ghost_pts_to r q v0)
+    (requires fun _ -> True)
+    (ensures fun _ _ _ -> v0 == v1)
+
+val ghost_read_pt (#a:Type) (#u:_) (#p:perm) (#v:erased a) (r:ghost_ref a)
+  : SteelSelGhost (erased a) u (ghost_pts_to r p v) (fun x -> ghost_pts_to r p x)
+           (requires fun _ -> True)
+           (ensures fun _ x _ -> x == v)
+
+val ghost_write_pt (#a:Type) (#u:_) (#v:erased a) (r:ghost_ref a) (x:erased a)
+  : SteelSelGhostT unit u
+    (ghost_pts_to r full_perm v)
+    (fun _ -> ghost_pts_to r full_perm x)
+
+(* Selector version of ghost references *)
+
+val ghost_ptr (#a: Type0) (r: ghost_ref a) : slprop u#1
 
 val ghost_ptr_sel (#a:Type0) (r:ghost_ref a) : selector a (ghost_ptr r)
 
 val ghost_ptr_sel_interp (#a:Type0) (r:ghost_ref a) (m:mem) : Lemma
   (requires interp (ghost_ptr r) m)
-  (ensures interp (R.ghost_pts_to r Steel.FractionalPermission.full_perm (ghost_ptr_sel r m)) m)
+  (ensures interp (ghost_pts_to_sl r full_perm (ghost_ptr_sel r m)) m)
 
 [@@ __steel_reduce__]
 let ghost_vptr' #a r : vprop' =
@@ -102,28 +257,30 @@ let ghost_vptr' #a r : vprop' =
 unfold
 let ghost_vptr r = VUnit (ghost_vptr' r)
 
-val ghost_alloc (#a:Type0) (#opened:inames) (x:Ghost.erased a) : SteelSelGhost (ghost_ref a) opened
+[@@ __steel_reduce__]
+let ghost_sel (#a:Type) (#p:vprop) (r:ghost_ref a)
+  (h:rmem p{FStar.Tactics.with_tactic selector_tactic (can_be_split p (ghost_vptr r) /\ True)})
+  = h (ghost_vptr r)
+
+val ghost_alloc (#a:Type0) (#opened:inames) (x:Ghost.erased a)
+  : SteelSelGhost (ghost_ref a) opened
   emp (fun r -> ghost_vptr r)
   (requires fun _ -> True)
-  (ensures fun _ r h1 -> h1 (ghost_vptr r) == Ghost.reveal x)
+  (ensures fun _ r h1 -> ghost_sel r h1 == Ghost.reveal x)
 
 val ghost_free (#a:Type0) (#opened:inames) (r:ghost_ref a) : SteelSelGhost unit opened
   (ghost_vptr r) (fun _ -> emp)
   (requires fun _ -> True)
   (ensures fun _ _ _ -> True)
 
-let ghost_read (#a:Type0) (#opened:inames) (r:ghost_ref a) : SteelSelGhost (Ghost.erased a) opened
-  (ghost_vptr r) (fun _ -> ghost_vptr r)
-  (requires fun _ -> True)
-  (ensures fun h0 x h1 -> h0 (ghost_vptr r) == h1 (ghost_vptr r) /\ Ghost.reveal x == h1 (ghost_vptr r))
-= gget (ghost_vptr r)
+val ghost_read (#a:Type0) (#opened:inames) (r:ghost_ref a)
+  : SteelSelGhost (Ghost.erased a) opened
+    (ghost_vptr r) (fun _ -> ghost_vptr r)
+    (requires fun _ -> True)
+    (ensures fun h0 x h1 -> h0 (ghost_vptr r) == h1 (ghost_vptr r) /\ Ghost.reveal x == h1 (ghost_vptr r))
 
-val ghost_write (#a:Type0) (#opened:inames) (r:ghost_ref a) (x:Ghost.erased a) : SteelSelGhost unit opened
-  (ghost_vptr r) (fun _ -> ghost_vptr r)
-  (requires fun _ -> True)
-  (ensures fun _ _ h1 -> Ghost.reveal x == h1 (ghost_vptr r))
-
-[@@ __steel_reduce__]
-let ghost_sel (#a:Type) (#p:vprop) (r:ghost_ref a)
-  (h:rmem p{FStar.Tactics.with_tactic selector_tactic (can_be_split p (ghost_vptr r) /\ True)})
-  = h (ghost_vptr r)
+val ghost_write (#a:Type0) (#opened:inames) (r:ghost_ref a) (x:Ghost.erased a)
+  : SteelSelGhost unit opened
+      (ghost_vptr r) (fun _ -> ghost_vptr r)
+      (requires fun _ -> True)
+      (ensures fun _ _ h1 -> Ghost.reveal x == h1 (ghost_vptr r))
